Fixing UseImmediate correctness proof and example

compiler/src/compiler/UseImmediateDef.v
@@ -1,22 +1,18 @@
 Require Import compiler.util.Common.
-(*
-Require Import compiler.FlattenExprDef. (* Only imported for testing UseImmediate *)
-Require Import compiler.StringNameGen. (* Only imported for testing UseImmediate *) *)
 Require Import compiler.FlatImp.
 Require Import Coq.Lists.List. Import ListNotations.
 Require Import bedrock2.Syntax.
 Require Import coqutil.Tactics.fwd.
 Require Import String.
-(* Open Scope string_scope. (* Only used for examples. *) *)
 Open Scope Z_scope.
 
-
+Local Notation var := String.string (only parsing).
 
 Section WithArgs.
   Context (is5BitImmediate : Z -> bool).
   Context (is12BitImmediate: Z -> bool).
 
-
+  Context {env: map.map String.string (list var * list var * stmt var)}.
 
   Fixpoint useImmediate(s: stmt string) : stmt string :=
     match s with
@@ -26,11 +22,7 @@ Section WithArgs.
     | SSeq s1 s2 =>
         let default := SSeq (useImmediate s1) (useImmediate s2) in
         match s1, s2 with
-        (*
-        | SSkip, _ => used2
-        | _, SSkip => used1 *)
         | SLit v1 l1, SOp v2 op v2a (Var v2b) =>
-
             match op with
             | Syntax.bopname.add
             | Syntax.bopname.and
@@ -62,78 +54,16 @@ Section WithArgs.
                                     else default
             | _ => default
             end
-        (*
-        | SLit v1 l1, SSeq (SLit v1b l1b) (SOp v2 op v2a (Var v2b)) =>
-            if (eqb v1 v1b) then default
-            else match op with
-            | Syntax.bopname.add
-            | Syntax.bopname.and
-            | Syntax.bopname.or
-            | Syntax.bopname.xor => if (is12BitImmediate l1) then
-                                      if eqb v1 v2b then
-                                        SSeq (SLit v1b l1b) (SOp v2 op v2a (Const l1))
-                                      else if eqb v1 v2a then
-                                             SSeq (SLit v1b l1b) (SOp v2 op v2b (Const l1))
-                                           else default
-                                    else default
-            | _ => default
-            end *)
         | _, _ => default
         end
     | _ => s
     end.
+
+  Definition useimmediate_function: (list string * list string * stmt string) -> result (list string * list string * stmt string) :=
+    fun '(argnames, retnames, body) =>
+      let body' := useImmediate body in
+      Success (argnames, retnames, body').
+
+  Definition useimmediate_functions : env -> result env :=
+    map.try_map_values useimmediate_function.
 End WithArgs.
-
-
-(*
-Following are examples for how UseImmediateDef works. Commented out for readability of compilation output. For now not using `Goal useImmediate (flatten_function ex_i) = expected_output because don't want to constrain expected output, what's more important is that whatever the output is is "correct" by semantics which would be shown by the proof in UseImmediate.v. To try out examples locally, uncomment here and in the imports at the start of the file.
-
-Definition ex0 := (["a"], [] : list string, Syntax.cmd.set "a" (Syntax.expr.op bopname.add (Syntax.expr.literal 1) (Syntax.expr.literal 16))).
-Definition ex1 := (["b"], ["a"], Syntax.cmd.set "b" (Syntax.expr.op bopname.slu (Syntax.expr.var "a") (Syntax.expr.literal 16))).
-Definition ex2 := (["b"], ["a"], Syntax.cmd.set "b" (Syntax.expr.op bopname.add (Syntax.expr.literal 1) (Syntax.expr.var "a"))).
-Definition ex3 := (["b"], ["a"], Syntax.cmd.set "b" (Syntax.expr.op bopname.ltu (Syntax.expr.var "a") (Syntax.expr.literal 16))).
-
-
-
-
-Definition sourceExs := [ex0; ex1; ex2; ex3].
-Definition unwrappedFlattenExs := let tmp :=  List.all_success (map flatten_function sourceExs) in
-                                  match tmp with
-                                  | Success l => l
-                                  | _ => []
-                                  end.
-Compute unwrappedFlattenExs.
-
-
-Definition useImmOnFlats (t: (list string * list string * stmt string)) : (list string * list string * stmt string)
-  := match t with
-     | (targs, trets, tstmt) => (targs, trets, (useImmediate (fun x => true) (fun x => true) tstmt))
-     end.
-
-Definition immediateExs := map useImmOnFlats unwrappedFlattenExs.
-
-(* Check that is5BitImmediate is used. *)
-Definition useImmOnFlats' (t: (list string * list string * stmt string)) : (list string * list string * stmt string)
-  := match t with
-     | (targs, trets, tstmt) => (targs, trets, (useImmediate (fun x => Z.ltb x 16) (fun x => true) tstmt))
-     end.
-
-Definition immediateExs' := map useImmOnFlats' unwrappedFlattenExs.
-
-
-
-(* Check that is12BitImmediate is used. *)
-Definition useImmOnFlats'' (t: (list string * list string * stmt string)) : (list string * list string * stmt string)
-  := match t with
-     | (targs, trets, tstmt) => (targs, trets, (useImmediate (fun x => true) (fun x => Z.ltb x 16) tstmt))
-     end.
-
-Definition immediateExs'' := map useImmOnFlats'' unwrappedFlattenExs.
-
-Compute unwrappedFlattenExs.
-(* For now, ex2 shouldn't be touched by this optimization, but could be touched after an earlier pass where superfluous SSkip's are removed. *)
-Compute immediateExs. (* All constants are small enough. *)
-Compute immediateExs'. (* is5BitImmediate is true only for < 16. *)
-Compute immediateExs''. (* is12BitImmediate is true only for < 16. *)
-
-*)
