compiler/src/compilerExamples/immediateExample.v
@@ -1,94 +1,63 @@
-Require Import Coq.Lists.List.
-Import ListNotations.
-Require bedrock2Examples.Demos.
-Require Import coqutil.Decidable.
 Require Import compiler.ExprImp.
-Require Import compiler.NameGen.
 Require Import compiler.Pipeline.
 Require Import riscv.Spec.Decode.
 Require Import riscv.Utility.Words32Naive.
 Require Import riscv.Utility.DefaultMemImpl32.
-Require Import riscv.Utility.Monads.
-Require Import compiler.util.Common.
-Require Import coqutil.Decidable.
 Require        riscv.Utility.InstructionNotations.
-Require Import riscv.Platform.MinimalLogging.
-Require Import bedrock2.MetricLogging.
-Require Import riscv.Platform.MetricMinimal.
-Require Import riscv.Utility.Utility.
 Require Import riscv.Utility.Encode.
 Require Import coqutil.Map.SortedList.
+Require        coqutil.Map.SortedListString.
 Require Import compiler.MemoryLayout.
-Require Import compiler.StringNameGen.
-Require Import riscv.Utility.InstructionCoercions.
-Require Import riscv.Platform.MetricRiscvMachine.
-Require bedrock2.Hexdump.
-Require Import bedrock2Examples.swap.
-Require Import bedrock2Examples.stackalloc.
-Require Import compilerExamples.SpillingTests.
-
+Require        riscv.Utility.bverify.
 Open Scope Z_scope.
 Open Scope string_scope.
 Open Scope ilist_scope.
 
-Definition var: Set := Z.
-Definition Reg: Set := Z.
-
-
-Local Existing Instance DefaultRiscvState.
-
 Local Instance funpos_env: map.map string Z := SortedListString.map _.
 
-Definition compile_ext_call(posenv: funpos_env)(mypos stackoffset: Z)(s: FlatImp.stmt Z) :=
-  match s with
-  | FlatImp.SInteract _ fname _ =>
-    if string_dec fname "nop" then
-      [[Addi Register0 Register0 0]]
-    else
-      nil
-  | _ => []
-  end.
+Definition compile_ext_call(posenv: funpos_env)(mypos stackoffset: Z)(s: FlatImp.stmt Z) : list Instruction := [].
 
-Notation RiscvMachine := MetricRiscvMachine.
+(* low_bound, hi_bound are expected inclusive bounds for UseImmediate optimization *)
+Definition test_imm_op(op: bopname.bopname)(low_bound: Z)(hi_bound: Z)
+  : (string * (list string * list string * cmd )) :=
+  (("main"),
+    (["a0"], ["ret_val"],
+      (cmd.seq (cmd.set "a0" (expr.op op (expr.var "a0")
+                                (expr.literal (low_bound - 1))))
+         (cmd.seq (cmd.set "a0" (expr.op op (expr.var "a0")
+                                   (expr.literal (low_bound))))
+            (cmd.seq (cmd.set "a0" (expr.op op (expr.var "a0")
+                                      (expr.literal (hi_bound))))
+               (cmd.set "ret_val" (expr.op op (expr.var "a0")
+                                     (expr.literal (hi_bound+1))))))))).
 
-Local Existing Instance coqutil.Map.SortedListString.map.
-Local Existing Instance coqutil.Map.SortedListString.ok.
-
-Definition main_stackalloc : (string * (list string * list string * cmd)) :=
-  ("main", ([]: list String.string, []: list String.string,
-                 cmd.stackalloc "x" 4 (cmd.stackalloc "y" 4 (cmd.call [] "imm_ex" [expr.var "x"; expr.var "y"])))).
-
-
-Definition immediate_example : (string * (list string * list string * cmd )) :=
-  ("imm_ex", ([]: list String.string, ["a"; "b"],
-                 cmd.seq (cmd.set "a" (expr.op bopname.sub (expr.literal 38) (expr.literal 31))) (cmd.set "b" (expr.op bopname.and (expr.var "a") (expr.literal 16))))).
-
-Definition allFuns: list (string * (list string * list string * cmd)) := [immediate_example; main_stackalloc].
-
-(* stack grows from high addreses to low addresses, first stack word will be written to
-   (stack_pastend-8), next stack word to (stack_pastend-16) etc *)
-Definition stack_pastend: Z := 2048.
-
-Lemma f_equal2: forall {A B: Type} {f1 f2: A -> B} {a1 a2: A},
-    f1 = f2 -> a1 = a2 -> f1 a1 = f2 a2.
-Proof. intros. congruence. Qed.
-
-Lemma f_equal3: forall {A B C: Type} {f1 f2: A -> B -> C} {a1 a2: A} {b1 b2: B},
-    f1 = f2 -> a1 = a2 -> b1 = b2 -> f1 a1 b1 = f2 a2 b2.
-Proof. intros. congruence. Qed.
-
-Lemma f_equal3_dep: forall {A B C: Type} {f1 f2: A -> B -> C} {a1 a2: A} {b1 b2: B},
-    f1 = f2 -> a1 = a2 -> b1 = b2 -> f1 a1 b1 = f2 a2 b2.
-Proof. intros. congruence. Qed.
-
+Definition imm_ex1 := test_imm_op bopname.add (-2048) (2047).
+Definition imm_ex2 := test_imm_op bopname.sub (-2047) (2048).
+Definition imm_ex3 := test_imm_op bopname.ltu (-2048) (2047).
+Definition imm_ex4 := test_imm_op bopname.lts (-2048) (2047).
+Definition imm_ex5 := test_imm_op bopname.srs 0 31.
+Definition imm_ex6 := test_imm_op bopname.slu 0 31.
 
 Local Instance RV32I_bitwidth: FlatToRiscvCommon.bitwidth_iset 32 RV32I.
 Proof. reflexivity. Qed.
 
-Definition imm_asm: list Instruction.
-  let r := eval cbv in (compile compile_ext_call allFuns) in set (res := r).
+Definition multi_compile funs_lists :=
+  List.all_success
+    (List.map
+       (fun x => '(insts, _, _) <- (compile compile_ext_call x) ;; Success insts) funs_lists).
+
+(* Expressing nested list literals as [[x]] is wonky
+   because of [[]] being used for list of Instructions *)
+Definition imm_asm: list (list Instruction).
+  let r := eval cbv in (multi_compile
+                          ([imm_ex1] ::
+                             [imm_ex2] ::
+                             [imm_ex3] ::
+                             [imm_ex4] ::
+                             [imm_ex5] ::
+                             [imm_ex6] :: [])) in set (res := r).
   match goal with
-  | res := Success (?x, _, _) |- _ => exact x
+  | res := Success (?x) |- _ => exact x
   end.
 Defined.
 
@@ -97,11 +66,12 @@ Module PrintAssembly.
   Goal True. let r := eval unfold imm_asm in imm_asm in idtac (* r *). Abort.
 End PrintAssembly.
 
-Definition imm_as_bytes: list Byte.byte := instrencode imm_asm.
-
-Module PrintBytes.
-  Import bedrock2.Hexdump.
-  Local Open Scope hexdump_scope.
-  Set Printing Width 100.
-  Goal True. let x := eval cbv in imm_as_bytes in idtac (* x *). Abort.
-End PrintBytes.
+Module CheckAssembly.
+  Goal Forall (bverify.validInstructions RV32I) imm_asm.
+    repeat (constructor; [solve
+                            [apply bverify.bvalidInstructions_valid;
+                             vm_compute; reflexivity]
+                         | ]).
+    constructor.
+  Qed.
+End CheckAssembly.
