compiler/src/compiler/UseImmediate.v
@@ -5,12 +5,15 @@ Require Import bedrock2.Syntax.
 Require Import coqutil.Tactics.fwd.
 Require Import String.
 Require Import compiler.UseImmediateDef.
+Require Import bedrock2.MetricLogging.
+
+Local Notation var := String.string (only parsing).
 
 Section WithArguments.
   Context {width : Z}.
   Context {BW :  Bitwidth.Bitwidth width }.
   Context {word :  word width } {word_ok : word.ok word}.
-  Context {env :  map.map string (list string * list string * stmt string) } {env_ok : map.ok env}.
+  Context {env :  map.map string (list var * list var * stmt var) } {env_ok : map.ok env}.
   Context {mem :  map.map word (Init.Byte.byte : Type) } {mem_ok: map.ok mem}.
   Context {locals :  map.map string word } {locals_ok: map.ok locals}.
   Context {ext_spec : Semantics.ExtSpec} {ext_spec_ok: Semantics.ext_spec.ok ext_spec}.
@@ -22,47 +25,70 @@ Section WithArguments.
        morphism (word.ring_morph (word := word)),
         constants [word_cst]).
 
-  Ltac destr_exec :=
-    match goal with
-    | [ |- exec _ (match ?x with | _ => _ end) _ _ _ _ _ ] => destr x
-    | [ |- exec _ (if ?x then _ else _ ) _ _ _ _ _ ] => destr x
-    end.
-
-  Ltac apply_exec :=
-   match goal with
-   | [ |- exec _ (SSeq _ _) _ _ _ _ _ ] => apply exec.seq_cps
-   | [ |- exec _ (SLit _ _) _ _ _ _ _ ] => apply exec.lit
-   end.
-
-  Ltac inversion_exec :=
-    match goal with
-    | [ H: exec _ _ _ _ _ _ _ |- _ ] => inversion H
-    end.
-
   Local Hint Constructors exec: core.
-  Lemma useImmediateCorrect :
-    forall e st t m l mc post, exec e st t m l mc post -> exec e (useImmediate is5BitImmediate is12BitImmediate st) t m l mc post.
-  Proof.
-  intros;
-  match goal with
-  | [ H: exec _ _ _ _ _ _ _  |- _ ] => induction H
-  end;
-  simpl in *; repeat destr_exec; eauto; inversion_exec;
-  match goal with
-  | [ H: ?P _ _ _ _, H0: forall t m l mc, ?P t m l mc -> _ |- _ ] => apply H0 in H; inversion H
-  end;
-  repeat apply_exec;
-  simpl in *;
-  match goal with
-  | [ H: map.get (map.put _ ?x _) ?x = _ |- _ ] => rewrite map.get_put_same in H; fwd
-  end;
-  eapply exec.op;  simpl;
-  eauto.
-  { rewrite word.add_comm. assumption. }
-  { replace (word.add y' (word.of_Z (- v)))  with  (word.sub  y' (word.of_Z v)) by ring. assumption. }
-  { rewrite word.and_comm. assumption. }
-  { rewrite word.or_comm. assumption. }
-  { rewrite word.xor_comm. assumption. }
-  Qed.
 
+  Lemma useImmediate_correct_aux:
+    forall eH eL,
+       (useimmediate_functions is5BitImmediate is12BitImmediate) eH = Success eL ->
+       forall sH t m mcH lH post,
+       exec eH sH t m lH mcH post ->
+       exec eL (useImmediate is5BitImmediate is12BitImmediate sH) t m lH mcH post.
+  Proof.
+    induction 2.
+    (* most cases stay the same *)
+    all: try solve [simpl; eauto].
+
+    (* SCall *)
+    { simpl.
+      eapply @exec.call; try eassumption.
+      assert (exists v2, (useimmediate_function is5BitImmediate is12BitImmediate) (params, rets, fbody) = Success v2 /\ map.get eL fname = Some v2).
+      { eapply map.try_map_values_fw.
+        - simpl in H; eapply H.
+        - eassumption.
+      }
+      destruct H5. destruct H5. simpl in H5. inversion H5. fwd.
+      eassumption.
+    }
+
+    (* SSeq *)
+    { simpl.
+      repeat (match goal with
+              | |- context[match ?x with _ => _ end] => destr x
+              | |- context[if ?x then _ else _ ] => destr x
+              end;
+              try solve [eapply @exec.seq; eassumption]);
+        simpl in *.
+
+      all: eapply @exec.seq_cps; eapply @exec.lit.
+
+      all: match goal with
+           | H: exec _ _ _ _ _ _ ?mid,
+               H': forall t m l mc,
+                 ?mid _ _ _ _ -> exec ?eL _ _ _ _ _ ?post
+                 |- _ => inversion H
+           end.
+
+      all: match goal with
+           | H: ?mid _ _ _ _,
+               H0: forall t m l mc,
+                 ?mid t m l mc -> exec ?eL _ _ _ _ _ ?post
+                 |- exec ?eL _ _ _ _ _ ?post
+             => apply H0 in H; inversion H
+           end.
+
+      all: simpl in *;
+        match goal with
+        | [ H: map.get (map.put _ ?x _) ?x = _ |- _ ]
+          => rewrite map.get_put_same in H; fwd
+        end.
+
+      all: eapply @exec.op; simpl in *; [ eassumption |  reflexivity | try eassumption ].
+
+      { rewrite word.add_comm. assumption. }
+      { replace (word.add y' (word.of_Z (- v)))  with  (word.sub  y' (word.of_Z v)) by ring. assumption. }
+      { rewrite word.and_comm. assumption. }
+      { rewrite word.or_comm. assumption. }
+      { rewrite word.xor_comm. assumption. }
+    }
+  Qed.
 End WithArguments.
